specs/Spec.CTR.fst
@@ -1,7 +1,10 @@
 module Spec.CTR
 
+open FStar.Mul
 open FStar.Seq
 open Spec.Lib
+
+#set-options "--max_fuel 0 --max_ifuel 0"
 
 type block_cipher_ctx = {
      keylen: nat ;
@@ -17,16 +20,16 @@ type counter (c:block_cipher_ctx) = UInt.uint_t c.counterbits
 type block_cipher (c:block_cipher_ctx) =  key c -> nonce c -> counter c -> block c
 
 val xor: #len:nat -> x:lbytes len -> y:lbytes len -> Tot (lbytes len)
-let xor #len x y = map2 (fun x y -> FStar.UInt8.(x ^^ y)) x y
+let xor #len x y = map2 FStar.UInt8.((^^)) x y
 
 val counter_mode: 
   ctx: block_cipher_ctx ->
   bc: block_cipher ctx ->
   k:key ctx -> n:nonce ctx -> c:counter ctx -> 
-  plain:seq UInt8.t{c + (length plain / ctx.blocklen) < pow2 ctx.counterbits} ->
+  plain:seq UInt8.t{c + ctx.incr * (length plain / ctx.blocklen) < pow2 ctx.counterbits} ->
   Tot (lbytes (length plain))
   (decreases (length plain))
-#reset-options "--z3rlimit 40 --max_fuel 2"
+#reset-options "--z3rlimit 200 --max_fuel 0 --max_ifuel 0"
 let rec counter_mode ctx block_enc key nonce counter plain =
   let len = length plain in 
   if len = 0 then Seq.createEmpty #UInt8.t else
@@ -41,4 +44,3 @@ let rec counter_mode ctx block_enc key nonce counter plain =
       let eb = xor b mask in
       let cipher = counter_mode ctx block_enc key nonce (counter + ctx.incr) plain in
       eb @| cipher 
-
