specs/Spec.Curve25519.fst
@@ -6,86 +6,61 @@ open FStar.UInt8
 open FStar.Endianness
 open Spec.Lib
 open Spec.Curve25519.Lemmas
-open Spec.AdditiveLaw
 
 #reset-options "--initial_fuel 0 --max_fuel 0 --z3rlimit 20"
 
 (* Field types and parameters *)
 let prime = pow2 255 - 19
-
 type elem : Type0 = e:int{e >= 0 /\ e < prime}
-
+let fadd e1 e2 = (e1 + e2) % prime
+let fsub e1 e2 = (e1 - e2) % prime
+let fmul e1 e2 = (e1 * e2) % prime
 let zero : elem = 0
 let one  : elem = 1
-
-val fadd: elem -> elem -> Tot elem
-let fadd e1 e2 = (e1 + e2) % prime
-let op_Plus_At e1 e2 = fadd e1 e2
-
-val fsub: elem -> elem -> Tot elem
-let fsub e1 e2 = (e1 - e2) % prime
-let op_Subtraction_At e1 e2 = fsub e1 e2
-
-val fmul: elem -> elem -> Tot elem
-let fmul e1 e2 = (e1 * e2) % prime
-let op_Star_At e1 e2 = fmul e1 e2
-
+(** Exponentiation *)
 let rec op_Star_Star (e:elem) (n:pos) : Tot elem (decreases n) =
   if n = 1 then e
-  else (
-    if n % 2 = 0 then op_Star_Star (e *@ e) (n / 2)
-    else e *@ (op_Star_Star (e *@ e) ((n-1)/2))
-  )
+  else
+    if n % 2 = 0 then op_Star_Star (e `fmul` e) (n / 2)
+    else e `fmul` (op_Star_Star (e `fmul` e) ((n-1)/2))
 
+(* Type aliases *)
 type scalar = lbytes 32
 type serialized_point = lbytes 32
-
 type proj_point = | Proj: x:elem -> z:elem -> proj_point
 
 let decodeScalar25519 (k:scalar) =
-  let k0  = index k 0  in
-  let k31 = index k 31 in
-  let k   = upd k 0 (k0 &^ 248uy)             in
-  let k   = upd k 31 ((k31 &^ 127uy) |^ 64uy) in
-  k
+  let k   = k.[0] <- (k.[0] &^ 248uy)          in
+  let k   = k.[31] <- ((k.[31] &^ 127uy) |^ 64uy) in k
 
 let decodePoint (u:serialized_point) =
   (little_endian u % pow2 255) % prime
 
 let add_and_double qx nq nqp1 =
   let x_1 = qx in
-  let x_2 = nq.x in 
-  let z_2 = nq.z in 
-  let x_3 = nqp1.x in 
-  let z_3 = nqp1.z in 
-  let a  = x_2 +@ z_2 in
+  let x_2, z_2 = nq.x, nq.z in 
+  let x_3, z_3 = nqp1.x, nqp1.z in 
+  let a  = x_2 `fadd` z_2 in
   let aa = a**2 in
-  let b  = x_2 -@ z_2 in
+  let b  = x_2 `fsub` z_2 in
   let bb = b**2 in
-  let e = aa -@ bb in
-  let c = x_3 +@ z_3 in
-  let d = x_3 -@ z_3 in
-  let da = d *@ a in
-  let cb = c *@ b in
-  let x_3 = (da +@ cb)**2 in
-  let z_3 = x_1 *@ ((da -@ cb)**2) in
-  let x_2 = aa *@ bb in
-  let z_2 = e *@ (aa +@ (121665 *@ e)) in
+  let e = aa `fsub` bb in
+  let c = x_3 `fadd` z_3 in
+  let d = x_3 `fsub` z_3 in
+  let da = d `fmul` a in
+  let cb = c `fmul` b in
+  let x_3 = (da `fadd` cb)**2 in
+  let z_3 = x_1 `fmul` ((da `fsub` cb)**2) in
+  let x_2 = aa `fmul` bb in
+  let z_2 = e `fmul` (aa `fadd` (121665 `fmul` e)) in
   Proj x_2 z_2, Proj x_3 z_3
 
 let ith_bit (k:scalar) (i:nat{i < 256}) =
   let q = i / 8 in let r = i % 8 in
-  (v (index k q) / pow2 r) % 2
+  (v (k.[q]) / pow2 r) % 2
 
-val montgomery_ladder_:
-  init:elem ->
-  x:proj_point ->
-  xp1:proj_point ->
-  k:scalar ->
-  ctr:nat{ctr <= 256} ->
-  Tot proj_point
-    (decreases ctr)
-let rec montgomery_ladder_ init x xp1 k ctr =
+let rec montgomery_ladder_ (init:elem) x xp1 (k:scalar) (ctr:nat{ctr<=256})
+  : Tot proj_point (decreases ctr) =
   if ctr = 0 then x
   else (
     let ctr' = ctr - 1 in
@@ -97,27 +72,23 @@ let rec montgomery_ladder_ init x xp1 k ctr =
     montgomery_ladder_ init x' xp1' k ctr'
   )
 
-
-val montgomery_ladder:
-  init:elem ->
-  k:scalar ->
-  Tot proj_point
-let montgomery_ladder init k =
+let montgomery_ladder (init:elem) (k:scalar) : Tot proj_point =
   montgomery_ladder_ init (Proj one zero) (Proj init one) k 256
 
-
 let encodePoint (p:proj_point) : Tot serialized_point =
-  let p = p.x *@ (p.z ** (prime - 2)) in
+  let p = p.x `fmul` (p.z ** (prime - 2)) in
   little_bytes 32ul p
 
-
-val scalarmult: k:scalar -> u:serialized_point -> Tot serialized_point
-let scalarmult k u =
+let scalarmult (k:scalar) (u:serialized_point) : Tot serialized_point =
   let k = decodeScalar25519 k in
   let u = decodePoint u in
   let res = montgomery_ladder u k in
   encodePoint res
 
+
+(* ********************* *)
+(* RFC 7748 Test Vectors *)
+(* ********************* *)
 
 let scalar1 = [
     0xa5uy; 0x46uy; 0xe3uy; 0x6buy; 0xf0uy; 0x52uy; 0x7cuy; 0x9duy;
